State_Networks.thy
@@ -243,26 +243,28 @@ definition
     by simp
 
   lemma collect_clki_prod_invariant:
-    "collect_clki prod_invariant = collect_clki (I' s)"
-    unfolding prod_invariant_def collect_clki_def
+    "Timed_Automata.collect_clki prod_invariant = Timed_Automata.collect_clki (I' s)"
+    unfolding prod_invariant_def Timed_Automata.collect_clki_def
     apply (simp split: prod.split)
     apply safe
      apply (subst (asm) I'_simp[where s' = s])
     by auto
 
   lemma collect_clki_prod_invariant':
-    "collect_clki prod_invariant \<subseteq> \<Union> {collect_clki (snd (fst A ! p)) | p. p < length (fst A)}"
+    "Timed_Automata.collect_clki prod_invariant
+    \<subseteq> \<Union> {Timed_Automata.collect_clki (snd (fst A ! p)) | p. p < length (fst A)}"
     unfolding collect_clki_prod_invariant[of s]
     unfolding inv_of_def Product_TA_Defs.product_ta_def
     unfolding Product_TA_Defs.product_invariant_def
     unfolding inv_of_def N_s_def
-    unfolding collect_clki_def
+    unfolding Timed_Automata.collect_clki_def
     unfolding collect_clock_pairs_def
     by auto
 
   lemma collect_clkt_prod_trans_subs:
-    "collect_clkt prod_trans \<subseteq> collect_clkt (\<Union> (T' ` UNIV))"
-    unfolding collect_clkt_def prod_trans_def prod_trans_i_def prod_trans_s_def by fastforce
+    "Timed_Automata.collect_clkt prod_trans \<subseteq> Timed_Automata.collect_clkt (\<Union> (T' ` UNIV))"
+    unfolding Timed_Automata.collect_clkt_def prod_trans_def prod_trans_i_def prod_trans_s_def
+    by fastforce
 
   lemma collect_clkvt_prod_trans_subs:
     "collect_clkvt prod_trans \<subseteq> collect_clkvt (\<Union> (T' ` UNIV))"
